examples/elliptic/arm/arm_rulesLib.sig
@@ -7,14 +7,10 @@ sig
     val REG_WRITEL_CONV      : conv
     val PSR_CONV             : conv
 
-    val all_arm_rules : (string * thm) list
     val arm_rules     : (string * thm) list
-    val nop_rules     : (string * thm) list
 
     val RULE_GET      : term -> thm list -> thm list
     val RULE_GET_ARM  : term -> thm
-    val RULE_GET_NOP  : term -> thm
 
     val GET_ARM       : string -> thm
-    val GET_NOP       : string -> thm
 end
